Simplify def. of CPU, add task precedence

identmp.v
@@ -1,25 +1,51 @@
 Require Import Vbase List job schedule priority platform.
 
-(* Mapping from processors to tasks at time t *)
-Definition processor_list := schedule -> cpu -> time -> job.
+Definition job_mapping := job -> processor_id -> time -> Prop.
 
-(* Whether a schedule is produced by an identical multiprocessor *)
-Definition ident_mp (num_cpus: nat) (hp: higher_priority) (cpumap: processor_list) (sched: schedule) :=
-
-  (* An identical multiprocessor has a fixed number of cpus *)
+(* Identical multiprocessor platform *)
+Definition ident_mp (num_cpus: nat) (hp: sched_job_hp_relation)
+                    (mapped: job_mapping) (sched: schedule) :=
+  (* The mapping has a finite number of cpus: [1, num_cpus) *)
   << mp_cpus_nonzero: num_cpus > 0 >> /\
-  << mp_num_cpus: forall t, length (cpumap sched t) = num_cpus >> /\
+  << mp_num_cpus: forall j cpu t, mapped j cpu t <-> cpu < num_cpus >> /\
 
   (* Job is scheduled iff it is mapped to a processor*)
-  << mp_mapping: forall j t, List.In (Some j) (cpumap sched t) <-> scheduled sched j t >> /\
+  << mp_mapping: forall j cpu t, scheduled sched j t <-> mapped j cpu t >> /\
 
   (* A job receives at most 1 unit of service *)
   << mp_max_service: forall j t, service_at sched j t <= 1 >> /\
 
   (* Global scheduling invariant *)
   << mp_invariant:
-       forall jlow t,
-         backlogged sched jlow t <->
-           (forall cpu, cpu < num_cpus ->
-             (exists (jhigh: job), hp sched t jhigh jlow
-                             /\ (nth cpu (cpumap sched t) None = Some jhigh))) >>.
+    forall jlow t, backlogged sched jlow t <->
+      (exists (j0: job), earlier_job sched j0 jlow /\ pending sched j0 t) \/
+      (forall cpu (MAXcpu: cpu < num_cpus),
+        exists jhigh, hp sched t jhigh jlow /\ mapped jhigh cpu t) >>.
+
+
+
+
+(*Require Export Coq.Structures.OrderedTypeEx.*)
+
+(* Just playing a bit with Finite Maps
+
+Module M := FMapList.Make(Nat_as_OT).
+Definition cpumap: Type := M.t job.
+Definition find k (m: cpumap) := M.find k m.
+Definition update (p: cpu * job) (m: cpumap) :=
+  M.add (fst p) (snd p) m.
+Notation "k |-> v" := (pair k v) (at level 60).
+Notation "[ ]" := (M.empty job).
+Notation "[ p1 , .. , pn ]" := (update p1 .. (update pn (M.empty job)) .. ).
+
+Variable job1 job2 job3: job.
+Variable mapped: time -> cpumap.
+
+Example ex1: find 3 [1 |-> job1, 3 |-> job2] = Some job2.
+Proof. reflexivity. Qed.
+
+Example ex2: find 2 [3 |-> job2] = None.
+Proof. reflexivity. Qed.
+
+(* Mapping from processors to tasks at time t *)
+Definition job_mapping := time -> cpumap.*)
